theories/cancellation/CancelCore.v
@@ -4,8 +4,8 @@ Require Import SModTr HModTr ModTr SMod HMod Mod.
 Require Import SimGlobal SimGTactics.
 Require Import SModCancel HModInline ElimRel CancelLib.
 
-Lemma cancel_aux_yield `{Σ: GRA} md
-  r ps pt srcs tgts cid st (rs rt rs0 rt0: Σ) l X (meta: X) Q ktrS ktrT
+Lemma cancel_aux_core `{Σ: GRA} md
+  r ps pt srcs tgts cid st (rs rt rs0 rt0: Σ) l X (meta: X) Q R ktrS ktrT
   (WFS: ✓ rs) (WFT: ✓ rt)
   (UPD: Own rs ==∗ Own rt)
   (LENS: cid < List.length srcs)
@@ -25,50 +25,28 @@ Lemma cancel_aux_yield `{Σ: GRA} md
       (∀ k x y, cid ≠ k → srcs !! k = Some x → tgts !! k = Some y → thread_rel md k x y)
       → CANCEL_GOAL md r rs0 rt0 ps pt srcs tgts cid st rs rt)
 
-  tid  
-  (SRC : srcs !! cid = Some (HModTr.trans (x <- trigger (Yield tid);; ktrS x)))
-  (TGT : tgts !! cid = Some (HModTr.trans (cancel_term md meta Q (x <- HoareYieldE tid;; ktrT x))))
+  (e: coreE R)
+  (SRC : srcs !! cid = Some (HModTr.trans (x <- trigger e;; ktrS x)))
+  (TGT : tgts !! cid = Some (HModTr.trans (cancel_term md meta Q (x <- trigger e;; ktrT x))))
   :
   CANCEL_GOAL md (gpaco7 _simg (cpn7 _simg) bot7 r) rs0 rt0 ps pt srcs tgts cid st rs rt.
 Proof.
   r.
-  ziter_l. rewrite SRC. ired. zstep_l.
-  ziter_r. rewrite TGT. ired. zstep_r.
-
-  destruct (Nat.eq_dec cid tid).
-  {
-    subst tid.
+  ziter_l. ziter_r. rewrite SRC TGT.
+  depdes e.
+  + zstep_r. zstep_r.
+    zstep_l. exists x. zstep_l.
     gstep. econs; econs; eauto using smj_lt_mid_top.
-    gbase. eapply CIH; zsimpl_len; et; zsimpl_len.
-    { zlookup_insert. ired. et. }
-    { zlookup_insert. ired. et. }
-    
-    intros k t1 t2 NEQ.
-    do 2 zlookup_insert_ne. i. eauto.
-  }
-
-  destruct (classic (tid < List.length srcs)); cycle 1.
-  {
-    ziter_l. zlookup_insert_ne.
-    rewrite lookup_ge_None_2; try nia.
-    zstep_l. unfold triggerUB. zstep_l.
-  }
-
-  exploit lookup_lt_is_Some_2; eauto. i. inv x0.
-  exploit (lookup_lt_is_Some_2 tgts tid); [nia|]. i. inv x1.
-  assert (tid < base.length tgts) by nia.
-  hexploit RELS; eauto. i.
-  depdes H3. subst.
-
-  gstep. econs; econs; eauto using smj_lt_mid_top.
-  gbase. eapply CIH; zsimpl_len; et; zsimpl_len.
-  { zlookup_insert_ne. ired. et. }
-  { zlookup_insert_ne. ired. et. }
-
-  i. destruct (Nat.eq_dec cid k); subst; cycle 1.
-  { revert H4 H5. do 2 zlookup_insert_ne. i. eauto. }
-
-  revert H4 H5. zlookup_insert. zlookup_insert. i. inv H5.
-  econs; grind; eauto.
+    gbase. eapply CIH; zsimpl_len; try zlookup_insert; et.
+    intros ? ? ? ?. do 2 zlookup_insert_ne. eauto.
+  + zstep_l. zstep_l.
+    zstep_r. exists x. zstep_r.
+    gstep. econs; econs; eauto using smj_lt_mid_top.
+    gbase. eapply CIH; zsimpl_len; try zlookup_insert; et.
+    intros ? ? ? ?. do 2 zlookup_insert_ne. eauto.
+  + zstep. zstep_l. zstep_r. subst.
+    gstep. econs; econs; eauto using smj_lt_mid_top.
+    gbase. eapply CIH; zsimpl_len; try zlookup_insert; et.
+    intros ? ? ? ?. do 2 zlookup_insert_ne. eauto.
 Unshelve. all: eauto.
 (*SLOW*)Admitted.
