theories/cancellation/CancelRet.v
@@ -1,12 +1,11 @@
 Require Import Common.
 From iris.proofmode Require Import proofmode.
 Require Import SModTr HModTr ModTr SMod HMod Mod.
-Require Import SimGlobal.
+Require Import SimGlobal SimGTactics.
 Require Import SModCancel HModInline ElimRel CancelLib.
-Require Import SimGTactics.
 
-Lemma cancel_aux_head `{Σ: GRA} md
-  r ps pt srcs tgts cid st (rs rt rs0 rt0: Σ) l X X0 (meta: X) P Q ktrS ktrT
+Lemma cancel_aux_ret `{Σ: GRA} md
+  r ps pt srcs tgts cid st (rs rt rs0 rt0: Σ) X (meta: X) Q
   (WFS: ✓ rs) (WFT: ✓ rt)
   (UPD: Own rs ==∗ Own rt)
   (LENS: cid < List.length srcs)
@@ -14,7 +13,6 @@ Lemma cancel_aux_head `{Σ: GRA} md
   (LEN: List.length srcs = Datatypes.length tgts)
   (RET: ∀ vret ret : Any.t, cid = 0 → Q meta vret ret ⊢ ⌜vret = ret⌝)
   (RELS: ∀ k x y, cid ≠ k → srcs !! k = Some x → tgts !! k = Some y → thread_rel md k x y)
-  (KTR: ∀ (m: X0) varg, paco3 (@elim_rel_def _ md _) bot3 ((existT X0 m) :: l) (ktrS varg) (ktrT (m, m, varg)))
   (CIH: ∀ rs rt srcs tgts cid st ps pt X (meta : X) Q itrS itrT l,
       ✓ rs → (Own rs ==∗ Own rt) →
       List.length srcs = List.length tgts →
@@ -26,52 +24,35 @@ Lemma cancel_aux_head `{Σ: GRA} md
       (∀ k x y, cid ≠ k → srcs !! k = Some x → tgts !! k = Some y → thread_rel md k x y)
       → CANCEL_GOAL md r rs0 rt0 ps pt srcs tgts cid st rs rt)
 
-  varg
-  (SRC : srcs !! cid = Some (HModTr.trans (tau;; ktrS varg)))
-  (TGT : tgts !! cid = Some (HModTr.trans (cancel_term md meta Q (x <- hmod_elim_head X0 P varg;; ktrT x))))
+  v
+  (SRC : srcs !! cid = Some (HModTr.trans (Ret v)))
+  (TGT : tgts !! cid = Some (HModTr.trans (cancel_term md meta Q (Ret v))))
   :
   CANCEL_GOAL md (gpaco7 _simg (cpn7 _simg) bot7 r) rs0 rt0 ps pt srcs tgts cid st rs rt.
 Proof.
   r.
-  ziter_l. rewrite SRC. ired. zstep_l.
-
-  ziter_r. rewrite TGT. ired. zstep_r. zstep_r.
+  ziter_l. rewrite SRC.
+  zonly_l.
+  des_ifs; cycle 1.
+  { unfold triggerUB. do 2 zstep_l. }
+  zshow.
+  zstep_l.
+  ziter_r. rewrite TGT. zstep_r. zstep_r.
   ziter_r. zstep_r.
+  ziter_r. zstep_r.
+  ziter_r. zstep_r. zstep_r.
   ziter_r. zstep_r. zstep_r.
   ziter_r. zstep_r.
   ziter_r. zstep_r.
-  ziter_r. zstep_r. zstep_r.
-  ziter_r. zstep_r. zstep_r.
   ziter_r. zstep_r.
   ziter_r. zstep_r.
-  ziter_r. zstep_r.
-  ziter_r. zstep_r.
-  ziter_r. zstep_r. exists x. zstep_r.
-  ziter_r. zstep_r.
-  ziter_r. zstep_r. exists varg. zstep_r.
-  ziter_r. zstep_r.
-  ziter_r. zstep_r.
+  zstep.
 
   hexploit (Own_bupd_split rt); i; des; eauto.
-  assert (VALID: ✓ (a1 ⋅ x1) ∧ (Own (a1 ⋅ x1) ==∗ P x varg x0 ∗ Own x1)).
-  { split.
-    - eapply Own_wand_valid with (a1 := rt); eauto.
-      iIntros "RT". iMod (H with "RT") as "[A X]". iModIntro.
-      iSplitL "A"; eauto. iApply H1; eauto.
-    - iIntros "[A X]". iFrame. iApply H0. eauto.
-  }
-
-  ziter_r. zstep_r. exists (a1 ⋅ x1). zstep_r.
-  ziter_r. zstep_r. exists VALID. zstep_r.
-  ziter_r. zstep_r.
-  ziter_r. zstep_r.
-  ziter_r. zstep_r.
-
-  gstep. econs; econs; eauto using smj_lt_mid_top.
-  gbase. eapply CIH; zsimpl_len; try zlookup_insert; ired; et.
-  { iIntros "RS". iMod (UPD with "RS") as "RS". iMod (H with "RS") as "[A1 A2]".
-    iSplitL "A1"; eauto. iApply H1. eauto.
-  }
-  { intros k t1 t2 NEQ. do 2 zlookup_insert_ne. i. eauto. }
+  depdes Heq. specialize (RET r0 x eq_refl).
+  eapply Own_pure_soundness with (a := a1).
+  + eapply Own_bupd_valid in H; eauto.
+    eapply cmra_valid_op_l; eauto.
+  + etrans; eauto.
 Unshelve. all: eauto.
 (*SLOW*)Admitted.
